{-# OPTIONS --safe #-}

module Surface.Theorems where

open import Relation.Binary.PropositionalEquality using (refl)

open import Surface.Syntax
open import Surface.Syntax.Membership
open import Surface.Derivations
open import Surface.Theorems.Helpers
open import Surface.Theorems.Thinning
open import Surface.Theorems.Substitution

τ∈Γ-⇒-Γ⊢τ : Γ ok
          → τ ∈ Γ at ι
          → Γ ⊢ τ
τ∈Γ-⇒-Γ⊢τ (TCTX-Bind δ τδ) (∈-zero refl) = twf-weakening δ τδ τδ
τ∈Γ-⇒-Γ⊢τ (TCTX-Bind δ τδ) (∈-suc refl ∈) = twf-weakening δ τδ (τ∈Γ-⇒-Γ⊢τ δ ∈)

-- Referred to as T-implies-TWF in the paper
Γ⊢ε⦂τ-⇒-Γ⊢τ : Γ ⊢ ε ⦂ τ
            → Γ ⊢ τ
Γ⊢ε⦂τ-⇒-Γ⊢τ (T-Unit Γok) = TWF-TrueRef Γok
Γ⊢ε⦂τ-⇒-Γ⊢τ (T-Var Γok ∈-prf) = τ∈Γ-⇒-Γ⊢τ Γok ∈-prf
Γ⊢ε⦂τ-⇒-Γ⊢τ (T-Abs arrδ _) = arrδ
Γ⊢ε⦂τ-⇒-Γ⊢τ (T-App δ₁ δ₂) = sub-Γ⊢τ-front δ₂ (arr-wf-⇒-cod-wf (Γ⊢ε⦂τ-⇒-Γ⊢τ δ₁))
Γ⊢ε⦂τ-⇒-Γ⊢τ (T-Case resδ _ _) = resδ
Γ⊢ε⦂τ-⇒-Γ⊢τ (T-Con _ _ adtτ) = adtτ
Γ⊢ε⦂τ-⇒-Γ⊢τ (T-Sub _ superδ _) = superδ
Γ⊢ε⦂τ-⇒-Γ⊢τ (T-RConv _ τ'δ _) = τ'δ
